examples/proofs/tagged_ptr/generated_code.v
@@ -15,92 +15,90 @@ Section code.
   Definition loc_8 : location_info := LocationInfo file_0 20 28 20 29.
   Definition loc_9 : location_info := LocationInfo file_0 20 33 20 34.
   Definition loc_12 : location_info := LocationInfo file_0 29 2 29 26.
-  Definition loc_13 : location_info := LocationInfo file_0 30 2 30 139.
-  Definition loc_14 : location_info := LocationInfo file_0 30 9 30 138.
+  Definition loc_13 : location_info := LocationInfo file_0 30 2 30 164.
+  Definition loc_14 : location_info := LocationInfo file_0 30 9 30 163.
   Definition loc_15 : location_info := LocationInfo file_0 30 35 30 38.
   Definition loc_16 : location_info := LocationInfo file_0 30 35 30 38.
-  Definition loc_17 : location_info := LocationInfo file_0 30 40 30 77.
-  Definition loc_18 : location_info := LocationInfo file_0 30 49 30 76.
-  Definition loc_19 : location_info := LocationInfo file_0 30 50 30 71.
-  Definition loc_20 : location_info := LocationInfo file_0 30 50 30 63.
-  Definition loc_21 : location_info := LocationInfo file_0 30 62 30 63.
-  Definition loc_22 : location_info := LocationInfo file_0 30 62 30 63.
-  Definition loc_23 : location_info := LocationInfo file_0 30 66 30 71.
-  Definition loc_24 : location_info := LocationInfo file_0 30 66 30 71.
-  Definition loc_25 : location_info := LocationInfo file_0 30 74 30 75.
-  Definition loc_26 : location_info := LocationInfo file_0 30 74 30 75.
-  Definition loc_27 : location_info := LocationInfo file_0 29 16 29 25.
+  Definition loc_17 : location_info := LocationInfo file_0 30 40 30 67.
+  Definition loc_18 : location_info := LocationInfo file_0 30 41 30 62.
+  Definition loc_19 : location_info := LocationInfo file_0 30 41 30 54.
+  Definition loc_20 : location_info := LocationInfo file_0 30 53 30 54.
+  Definition loc_21 : location_info := LocationInfo file_0 30 53 30 54.
+  Definition loc_22 : location_info := LocationInfo file_0 30 57 30 62.
+  Definition loc_23 : location_info := LocationInfo file_0 30 57 30 62.
+  Definition loc_24 : location_info := LocationInfo file_0 30 65 30 66.
+  Definition loc_25 : location_info := LocationInfo file_0 30 65 30 66.
+  Definition loc_26 : location_info := LocationInfo file_0 29 16 29 25.
+  Definition loc_27 : location_info := LocationInfo file_0 29 16 29 22.
   Definition loc_28 : location_info := LocationInfo file_0 29 16 29 22.
-  Definition loc_29 : location_info := LocationInfo file_0 29 16 29 22.
+  Definition loc_29 : location_info := LocationInfo file_0 29 23 29 24.
   Definition loc_30 : location_info := LocationInfo file_0 29 23 29 24.
-  Definition loc_31 : location_info := LocationInfo file_0 29 23 29 24.
-  Definition loc_36 : location_info := LocationInfo file_0 39 2 39 19.
-  Definition loc_37 : location_info := LocationInfo file_0 39 9 39 18.
+  Definition loc_35 : location_info := LocationInfo file_0 39 2 39 19.
+  Definition loc_36 : location_info := LocationInfo file_0 39 9 39 18.
+  Definition loc_37 : location_info := LocationInfo file_0 39 9 39 12.
   Definition loc_38 : location_info := LocationInfo file_0 39 9 39 12.
-  Definition loc_39 : location_info := LocationInfo file_0 39 9 39 12.
+  Definition loc_39 : location_info := LocationInfo file_0 39 13 39 14.
   Definition loc_40 : location_info := LocationInfo file_0 39 13 39 14.
-  Definition loc_41 : location_info := LocationInfo file_0 39 13 39 14.
-  Definition loc_42 : location_info := LocationInfo file_0 39 16 39 17.
-  Definition loc_45 : location_info := LocationInfo file_0 48 2 48 30.
-  Definition loc_46 : location_info := LocationInfo file_0 49 2 49 121.
-  Definition loc_47 : location_info := LocationInfo file_0 49 9 49 120.
+  Definition loc_41 : location_info := LocationInfo file_0 39 16 39 17.
+  Definition loc_44 : location_info := LocationInfo file_0 48 2 48 30.
+  Definition loc_45 : location_info := LocationInfo file_0 49 2 49 137.
+  Definition loc_46 : location_info := LocationInfo file_0 49 9 49 136.
+  Definition loc_47 : location_info := LocationInfo file_0 49 35 49 38.
   Definition loc_48 : location_info := LocationInfo file_0 49 35 49 38.
-  Definition loc_49 : location_info := LocationInfo file_0 49 35 49 38.
-  Definition loc_50 : location_info := LocationInfo file_0 49 40 49 68.
-  Definition loc_51 : location_info := LocationInfo file_0 49 49 49 67.
-  Definition loc_52 : location_info := LocationInfo file_0 49 50 49 51.
-  Definition loc_53 : location_info := LocationInfo file_0 49 50 49 51.
-  Definition loc_54 : location_info := LocationInfo file_0 49 54 49 66.
-  Definition loc_55 : location_info := LocationInfo file_0 49 54 49 55.
-  Definition loc_56 : location_info := LocationInfo file_0 49 54 49 55.
-  Definition loc_57 : location_info := LocationInfo file_0 49 58 49 66.
-  Definition loc_58 : location_info := LocationInfo file_0 49 59 49 60.
-  Definition loc_59 : location_info := LocationInfo file_0 49 64 49 65.
-  Definition loc_60 : location_info := LocationInfo file_0 48 16 48 29.
-  Definition loc_61 : location_info := LocationInfo file_0 48 28 48 29.
-  Definition loc_62 : location_info := LocationInfo file_0 48 28 48 29.
-  Definition loc_67 : location_info := LocationInfo file_0 54 2 54 15.
-  Definition loc_68 : location_info := LocationInfo file_0 56 2 56 24.
-  Definition loc_69 : location_info := LocationInfo file_0 57 2 57 26.
-  Definition loc_70 : location_info := LocationInfo file_0 59 2 59 36.
-  Definition loc_71 : location_info := LocationInfo file_0 60 2 60 13.
-  Definition loc_72 : location_info := LocationInfo file_0 60 9 60 12.
-  Definition loc_73 : location_info := LocationInfo file_0 60 9 60 12.
-  Definition loc_74 : location_info := LocationInfo file_0 60 10 60 12.
-  Definition loc_75 : location_info := LocationInfo file_0 60 10 60 12.
-  Definition loc_76 : location_info := LocationInfo file_0 59 15 59 35.
-  Definition loc_77 : location_info := LocationInfo file_0 59 26 59 35.
-  Definition loc_78 : location_info := LocationInfo file_0 59 26 59 31.
-  Definition loc_79 : location_info := LocationInfo file_0 59 26 59 31.
-  Definition loc_80 : location_info := LocationInfo file_0 59 32 59 34.
-  Definition loc_81 : location_info := LocationInfo file_0 59 32 59 34.
-  Definition loc_84 : location_info := LocationInfo file_0 57 9 57 24.
-  Definition loc_85 : location_info := LocationInfo file_0 57 9 57 19.
-  Definition loc_86 : location_info := LocationInfo file_0 57 9 57 15.
-  Definition loc_87 : location_info := LocationInfo file_0 57 9 57 15.
-  Definition loc_88 : location_info := LocationInfo file_0 57 16 57 18.
-  Definition loc_89 : location_info := LocationInfo file_0 57 16 57 18.
-  Definition loc_90 : location_info := LocationInfo file_0 57 23 57 24.
-  Definition loc_91 : location_info := LocationInfo file_0 56 13 56 23.
-  Definition loc_92 : location_info := LocationInfo file_0 56 13 56 16.
-  Definition loc_93 : location_info := LocationInfo file_0 56 13 56 16.
-  Definition loc_94 : location_info := LocationInfo file_0 56 17 56 19.
-  Definition loc_95 : location_info := LocationInfo file_0 56 18 56 19.
-  Definition loc_96 : location_info := LocationInfo file_0 56 21 56 22.
-  Definition loc_99 : location_info := LocationInfo file_0 54 13 54 14.
-  Definition loc_104 : location_info := LocationInfo file_0 69 2 69 30.
-  Definition loc_105 : location_info := LocationInfo file_0 70 2 70 27.
-  Definition loc_106 : location_info := LocationInfo file_0 70 9 70 26.
-  Definition loc_107 : location_info := LocationInfo file_0 70 9 70 21.
-  Definition loc_108 : location_info := LocationInfo file_0 70 9 70 10.
-  Definition loc_109 : location_info := LocationInfo file_0 70 9 70 10.
-  Definition loc_110 : location_info := LocationInfo file_0 70 13 70 21.
-  Definition loc_111 : location_info := LocationInfo file_0 70 14 70 15.
-  Definition loc_112 : location_info := LocationInfo file_0 70 19 70 20.
-  Definition loc_113 : location_info := LocationInfo file_0 70 25 70 26.
-  Definition loc_114 : location_info := LocationInfo file_0 69 16 69 29.
-  Definition loc_115 : location_info := LocationInfo file_0 69 28 69 29.
-  Definition loc_116 : location_info := LocationInfo file_0 69 28 69 29.
+  Definition loc_49 : location_info := LocationInfo file_0 49 40 49 58.
+  Definition loc_50 : location_info := LocationInfo file_0 49 41 49 42.
+  Definition loc_51 : location_info := LocationInfo file_0 49 41 49 42.
+  Definition loc_52 : location_info := LocationInfo file_0 49 45 49 57.
+  Definition loc_53 : location_info := LocationInfo file_0 49 45 49 46.
+  Definition loc_54 : location_info := LocationInfo file_0 49 45 49 46.
+  Definition loc_55 : location_info := LocationInfo file_0 49 49 49 57.
+  Definition loc_56 : location_info := LocationInfo file_0 49 50 49 51.
+  Definition loc_57 : location_info := LocationInfo file_0 49 55 49 56.
+  Definition loc_58 : location_info := LocationInfo file_0 48 16 48 29.
+  Definition loc_59 : location_info := LocationInfo file_0 48 28 48 29.
+  Definition loc_60 : location_info := LocationInfo file_0 48 28 48 29.
+  Definition loc_65 : location_info := LocationInfo file_0 54 2 54 15.
+  Definition loc_66 : location_info := LocationInfo file_0 56 2 56 24.
+  Definition loc_67 : location_info := LocationInfo file_0 57 2 57 26.
+  Definition loc_68 : location_info := LocationInfo file_0 59 2 59 36.
+  Definition loc_69 : location_info := LocationInfo file_0 60 2 60 13.
+  Definition loc_70 : location_info := LocationInfo file_0 60 9 60 12.
+  Definition loc_71 : location_info := LocationInfo file_0 60 9 60 12.
+  Definition loc_72 : location_info := LocationInfo file_0 60 10 60 12.
+  Definition loc_73 : location_info := LocationInfo file_0 60 10 60 12.
+  Definition loc_74 : location_info := LocationInfo file_0 59 15 59 35.
+  Definition loc_75 : location_info := LocationInfo file_0 59 26 59 35.
+  Definition loc_76 : location_info := LocationInfo file_0 59 26 59 31.
+  Definition loc_77 : location_info := LocationInfo file_0 59 26 59 31.
+  Definition loc_78 : location_info := LocationInfo file_0 59 32 59 34.
+  Definition loc_79 : location_info := LocationInfo file_0 59 32 59 34.
+  Definition loc_82 : location_info := LocationInfo file_0 57 9 57 24.
+  Definition loc_83 : location_info := LocationInfo file_0 57 9 57 19.
+  Definition loc_84 : location_info := LocationInfo file_0 57 9 57 15.
+  Definition loc_85 : location_info := LocationInfo file_0 57 9 57 15.
+  Definition loc_86 : location_info := LocationInfo file_0 57 16 57 18.
+  Definition loc_87 : location_info := LocationInfo file_0 57 16 57 18.
+  Definition loc_88 : location_info := LocationInfo file_0 57 23 57 24.
+  Definition loc_89 : location_info := LocationInfo file_0 56 13 56 23.
+  Definition loc_90 : location_info := LocationInfo file_0 56 13 56 16.
+  Definition loc_91 : location_info := LocationInfo file_0 56 13 56 16.
+  Definition loc_92 : location_info := LocationInfo file_0 56 17 56 19.
+  Definition loc_93 : location_info := LocationInfo file_0 56 18 56 19.
+  Definition loc_94 : location_info := LocationInfo file_0 56 21 56 22.
+  Definition loc_97 : location_info := LocationInfo file_0 54 13 54 14.
+  Definition loc_102 : location_info := LocationInfo file_0 69 2 69 30.
+  Definition loc_103 : location_info := LocationInfo file_0 70 2 70 27.
+  Definition loc_104 : location_info := LocationInfo file_0 70 9 70 26.
+  Definition loc_105 : location_info := LocationInfo file_0 70 9 70 21.
+  Definition loc_106 : location_info := LocationInfo file_0 70 9 70 10.
+  Definition loc_107 : location_info := LocationInfo file_0 70 9 70 10.
+  Definition loc_108 : location_info := LocationInfo file_0 70 13 70 21.
+  Definition loc_109 : location_info := LocationInfo file_0 70 14 70 15.
+  Definition loc_110 : location_info := LocationInfo file_0 70 19 70 20.
+  Definition loc_111 : location_info := LocationInfo file_0 70 25 70 26.
+  Definition loc_112 : location_info := LocationInfo file_0 69 16 69 29.
+  Definition loc_113 : location_info := LocationInfo file_0 69 28 69 29.
+  Definition loc_114 : location_info := LocationInfo file_0 69 28 69 29.
 
   (* Definition of function [tag_of]. *)
   Definition impl_tag_of : function := {|
@@ -131,9 +129,9 @@ Section code.
     f_code := (
       <[ "#0" :=
         "old_t" <-{ it_layout u8 }
-          LocInfoE loc_27 (Call (LocInfoE loc_29 (global_tag_of)) [@{expr} LocInfoE loc_30 (use{void*} (LocInfoE loc_31 ("p"))) ]) ;
+          LocInfoE loc_26 (Call (LocInfoE loc_28 (global_tag_of)) [@{expr} LocInfoE loc_29 (use{void*} (LocInfoE loc_30 ("p"))) ]) ;
         locinfo: loc_13 ;
-        Return (LocInfoE loc_14 (CopyAllocId (PtrOp) (LocInfoE loc_17 (UnOp (CastOp $ PtrOp) (IntOp uintptr_t) (LocInfoE loc_18 ((LocInfoE loc_19 ((LocInfoE loc_20 (UnOp (CastOp $ IntOp uintptr_t) (PtrOp) (LocInfoE loc_21 (use{void*} (LocInfoE loc_22 ("p")))))) -{IntOp uintptr_t, IntOp uintptr_t} (LocInfoE loc_23 (UnOp (CastOp $ IntOp uintptr_t) (IntOp u8) (LocInfoE loc_23 (use{it_layout u8} (LocInfoE loc_24 ("old_t")))))))) +{IntOp uintptr_t, IntOp uintptr_t} (LocInfoE loc_25 (UnOp (CastOp $ IntOp uintptr_t) (IntOp u8) (LocInfoE loc_25 (use{it_layout u8} (LocInfoE loc_26 ("t")))))))))) (LocInfoE loc_15 (use{void*} (LocInfoE loc_16 ("p"))))))
+        Return (LocInfoE loc_14 (CopyAllocId (IntOp uintptr_t) (LocInfoE loc_17 ((LocInfoE loc_18 ((LocInfoE loc_19 (UnOp (CastOp $ IntOp uintptr_t) (PtrOp) (LocInfoE loc_20 (use{void*} (LocInfoE loc_21 ("p")))))) -{IntOp uintptr_t, IntOp uintptr_t} (LocInfoE loc_22 (UnOp (CastOp $ IntOp uintptr_t) (IntOp u8) (LocInfoE loc_22 (use{it_layout u8} (LocInfoE loc_23 ("old_t")))))))) +{IntOp uintptr_t, IntOp uintptr_t} (LocInfoE loc_24 (UnOp (CastOp $ IntOp uintptr_t) (IntOp u8) (LocInfoE loc_24 (use{it_layout u8} (LocInfoE loc_25 ("t")))))))) (LocInfoE loc_15 (use{void*} (LocInfoE loc_16 ("p"))))))
       ]> $∅
     )%E
   |}.
@@ -148,9 +146,9 @@ Section code.
     f_init := "#0";
     f_code := (
       <[ "#0" :=
-        locinfo: loc_36 ;
-        Return (LocInfoE loc_37 (Call (LocInfoE loc_39 (global_tag)) [@{expr} LocInfoE loc_40 (use{void*} (LocInfoE loc_41 ("p"))) ;
-               LocInfoE loc_42 (UnOp (CastOp $ IntOp u8) (IntOp i32) (LocInfoE loc_42 (i2v 0 i32))) ]))
+        locinfo: loc_35 ;
+        Return (LocInfoE loc_36 (Call (LocInfoE loc_38 (global_tag)) [@{expr} LocInfoE loc_39 (use{void*} (LocInfoE loc_40 ("p"))) ;
+               LocInfoE loc_41 (UnOp (CastOp $ IntOp u8) (IntOp i32) (LocInfoE loc_41 (i2v 0 i32))) ]))
       ]> $∅
     )%E
   |}.
@@ -167,9 +165,9 @@ Section code.
     f_code := (
       <[ "#0" :=
         "i" <-{ it_layout uintptr_t }
-          LocInfoE loc_60 (UnOp (CastOp $ IntOp uintptr_t) (PtrOp) (LocInfoE loc_61 (use{void*} (LocInfoE loc_62 ("p"))))) ;
-        locinfo: loc_46 ;
-        Return (LocInfoE loc_47 (CopyAllocId (PtrOp) (LocInfoE loc_50 (UnOp (CastOp $ PtrOp) (IntOp uintptr_t) (LocInfoE loc_51 ((LocInfoE loc_52 (use{it_layout uintptr_t} (LocInfoE loc_53 ("i")))) -{IntOp uintptr_t, IntOp uintptr_t} (LocInfoE loc_54 ((LocInfoE loc_55 (use{it_layout uintptr_t} (LocInfoE loc_56 ("i")))) %{IntOp uintptr_t, IntOp uintptr_t} (LocInfoE loc_57 (UnOp (CastOp $ IntOp uintptr_t) (IntOp i32) (LocInfoE loc_57 ((LocInfoE loc_58 (i2v 1 i32)) <<{IntOp i32, IntOp i32} (LocInfoE loc_59 (i2v 3 i32)))))))))))) (LocInfoE loc_48 (use{void*} (LocInfoE loc_49 ("p"))))))
+          LocInfoE loc_58 (UnOp (CastOp $ IntOp uintptr_t) (PtrOp) (LocInfoE loc_59 (use{void*} (LocInfoE loc_60 ("p"))))) ;
+        locinfo: loc_45 ;
+        Return (LocInfoE loc_46 (CopyAllocId (IntOp uintptr_t) (LocInfoE loc_49 ((LocInfoE loc_50 (use{it_layout uintptr_t} (LocInfoE loc_51 ("i")))) -{IntOp uintptr_t, IntOp uintptr_t} (LocInfoE loc_52 ((LocInfoE loc_53 (use{it_layout uintptr_t} (LocInfoE loc_54 ("i")))) %{IntOp uintptr_t, IntOp uintptr_t} (LocInfoE loc_55 (UnOp (CastOp $ IntOp uintptr_t) (IntOp i32) (LocInfoE loc_55 ((LocInfoE loc_56 (i2v 1 i32)) <<{IntOp i32, IntOp i32} (LocInfoE loc_57 (i2v 3 i32)))))))))) (LocInfoE loc_47 (use{void*} (LocInfoE loc_48 ("p"))))))
       ]> $∅
     )%E
   |}.
@@ -187,16 +185,16 @@ Section code.
     f_code := (
       <[ "#0" :=
         "x" <-{ it_layout size_t }
-          LocInfoE loc_99 (UnOp (CastOp $ IntOp size_t) (IntOp i32) (LocInfoE loc_99 (i2v 0 i32))) ;
+          LocInfoE loc_97 (UnOp (CastOp $ IntOp size_t) (IntOp i32) (LocInfoE loc_97 (i2v 0 i32))) ;
         "tp" <-{ void* }
-          LocInfoE loc_91 (Call (LocInfoE loc_93 (global_tag)) [@{expr} LocInfoE loc_94 (&(LocInfoE loc_95 ("x"))) ;
-          LocInfoE loc_96 (UnOp (CastOp $ IntOp u8) (IntOp i32) (LocInfoE loc_96 (i2v 1 i32))) ]) ;
-        locinfo: loc_69 ;
-        assert: (LocInfoE loc_84 (UnOp (CastOp $ IntOp bool_it) (IntOp i32) (LocInfoE loc_84 ((LocInfoE loc_85 (UnOp (CastOp $ IntOp i32) (IntOp u8) (LocInfoE loc_85 (Call (LocInfoE loc_87 (global_tag_of)) [@{expr} LocInfoE loc_88 (use{void*} (LocInfoE loc_89 ("tp"))) ])))) ={IntOp i32, IntOp i32} (LocInfoE loc_90 (i2v 1 i32)))))) ;
+          LocInfoE loc_89 (Call (LocInfoE loc_91 (global_tag)) [@{expr} LocInfoE loc_92 (&(LocInfoE loc_93 ("x"))) ;
+          LocInfoE loc_94 (UnOp (CastOp $ IntOp u8) (IntOp i32) (LocInfoE loc_94 (i2v 1 i32))) ]) ;
+        locinfo: loc_67 ;
+        assert: (LocInfoE loc_82 (UnOp (CastOp $ IntOp bool_it) (IntOp i32) (LocInfoE loc_82 ((LocInfoE loc_83 (UnOp (CastOp $ IntOp i32) (IntOp u8) (LocInfoE loc_83 (Call (LocInfoE loc_85 (global_tag_of)) [@{expr} LocInfoE loc_86 (use{void*} (LocInfoE loc_87 ("tp"))) ])))) ={IntOp i32, IntOp i32} (LocInfoE loc_88 (i2v 1 i32)))))) ;
         "px" <-{ void* }
-          LocInfoE loc_76 (UnOp (CastOp $ PtrOp) (PtrOp) (LocInfoE loc_77 (Call (LocInfoE loc_79 (global_untag)) [@{expr} LocInfoE loc_80 (use{void*} (LocInfoE loc_81 ("tp"))) ]))) ;
-        locinfo: loc_71 ;
-        Return (LocInfoE loc_72 (use{it_layout size_t} (LocInfoE loc_74 (!{void*} (LocInfoE loc_75 ("px"))))))
+          LocInfoE loc_74 (UnOp (CastOp $ PtrOp) (PtrOp) (LocInfoE loc_75 (Call (LocInfoE loc_77 (global_untag)) [@{expr} LocInfoE loc_78 (use{void*} (LocInfoE loc_79 ("tp"))) ]))) ;
+        locinfo: loc_69 ;
+        Return (LocInfoE loc_70 (use{it_layout size_t} (LocInfoE loc_72 (!{void*} (LocInfoE loc_73 ("px"))))))
       ]> $∅
     )%E
   |}.
@@ -213,9 +211,9 @@ Section code.
     f_code := (
       <[ "#0" :=
         "i" <-{ it_layout uintptr_t }
-          LocInfoE loc_114 (UnOp (CastOp $ IntOp uintptr_t) (PtrOp) (LocInfoE loc_115 (use{void*} (LocInfoE loc_116 ("p"))))) ;
-        locinfo: loc_105 ;
-        Return (LocInfoE loc_106 ((LocInfoE loc_107 ((LocInfoE loc_108 (use{it_layout uintptr_t} (LocInfoE loc_109 ("i")))) %{IntOp uintptr_t, IntOp uintptr_t} (LocInfoE loc_110 (UnOp (CastOp $ IntOp uintptr_t) (IntOp i32) (LocInfoE loc_110 ((LocInfoE loc_111 (i2v 1 i32)) <<{IntOp i32, IntOp i32} (LocInfoE loc_112 (i2v 3 i32)))))))) ={IntOp uintptr_t, IntOp uintptr_t} (LocInfoE loc_113 (UnOp (CastOp $ IntOp uintptr_t) (IntOp i32) (LocInfoE loc_113 (i2v 0 i32))))))
+          LocInfoE loc_112 (UnOp (CastOp $ IntOp uintptr_t) (PtrOp) (LocInfoE loc_113 (use{void*} (LocInfoE loc_114 ("p"))))) ;
+        locinfo: loc_103 ;
+        Return (LocInfoE loc_104 ((LocInfoE loc_105 ((LocInfoE loc_106 (use{it_layout uintptr_t} (LocInfoE loc_107 ("i")))) %{IntOp uintptr_t, IntOp uintptr_t} (LocInfoE loc_108 (UnOp (CastOp $ IntOp uintptr_t) (IntOp i32) (LocInfoE loc_108 ((LocInfoE loc_109 (i2v 1 i32)) <<{IntOp i32, IntOp i32} (LocInfoE loc_110 (i2v 3 i32)))))))) ={IntOp uintptr_t, IntOp uintptr_t} (LocInfoE loc_111 (UnOp (CastOp $ IntOp uintptr_t) (IntOp i32) (LocInfoE loc_111 (i2v 0 i32))))))
       ]> $∅
     )%E
   |}.
