theories/typing/automation/loc_eq.v
@@ -51,6 +51,9 @@ Inductive FICLocSemantic : Set :=.
 Global Instance find_in_context_type_loc_semantic_inst `{!typeG Σ} l :
   FindInContext (FindLoc l) 2%nat FICLocSemantic :=
   λ T, i2p (find_in_context_type_loc_id l T).
+Global Instance find_in_context_type_val_P_loc_semantic_inst `{!typeG Σ} (l : loc) :
+  FindInContext (FindValP l) 2%nat FICLocSemantic :=
+  λ T, i2p (find_in_context_type_val_P_loc_id l T).
 Global Instance find_in_context_loc_in_bounds_semantic_inst `{!typeG Σ} l :
   FindInContext (FindLocInBounds l) 2%nat FICLocSemantic :=
   λ T, i2p (find_in_context_loc_in_bounds l T).
